**Interviewer**: Let's discuss a problem where we build a table of `n` rows. We start by writing `0` in the `1st` row. In every subsequent row, each occurrence of `0` is replaced with `01`, and each occurrence of `1` is replaced with `10`. Given two integers `n` and `k`, your task is to return the `kth` (1-indexed) symbol in the `nth` row of the table.

To make it clearer, here are a few examples:
- For `n = 3`, the rows in the table would be:
  - Row 1: `0`
  - Row 2: `01`
  - Row 3: `0110`

For `n = 1, k = 1`, the output should be `0`.
For `n = 2, k = 1`, the output should be `0`.
For `n = 2, k = 2`, the output should be `1`.

**Interviewer**: Can you think of a brute-force approach to solve this problem?

---

**Interviewee**: Sure, the brute-force approach would be to generate each row from the first row up to the nth row, and then return the kth element of the nth row. Let me outline the steps:

1. Start with the first row: `row = "0"`.
2. For each subsequent row up to `n`, create a new row by replacing each `0` in the current row with `01` and each `1` with `10`.
3. After generating the `nth` row, return the element at position `k-1` (since k is 1-indexed).

**Interviewer**: Yes, that's the right approach for brute force. What would be the time and space complexity of this brute-force approach?

**Interviewee**: 
- **Time Complexity**: As each row is generated based on the previous row, the length of the rows doubles each time. Therefore, the length of the nth row is \(2^{n-1}\). Generating each row takes \(O(2^{n-1})\) time. Summing this up for all rows gives us \(O(1 + 2 + 4 + \ldots + 2^{n-1}) = O(2^n)\).
- **Space Complexity**: Similarly, the space needed to store up to the nth row is \(O(2^{n-1})\) due to the doubling length of each row.

**Interviewer**: Great analysis. The brute-force approach is understandable but not feasible for larger `n` due to exponential growth. Can we optimize this?

**Interviewee**: Yes, we can optimize this problem using a recursive or mathematical approach instead of constructing all rows. The key insight is that the symbol's generation pattern is recursive, and we can determine the kth symbol based on the previous row's symbols.

**Interviewer**: Can you explain this approach in detail?

---

**Interviewee**: Certainly! Here's the optimized approach:

1. Notice that each row is generated by alternating patterns of the previous row, meaning:
   - If we know the symbol at position `k` in the `n`th row, it is determined by the symbol at position \( \left\lceil \frac{k}{2} \right\rceil \) in the `n-1`th row.
   - If `k` is odd, the symbol is the same as the symbol in the previous row at position \( \left\lceil \frac{k}{2} \right\rceil \).
   - If `k` is even, the symbol is the complement (0 becomes 1, and 1 becomes 0) of the symbol at position \( \left\lceil \frac{k}{2} \right\rceil \) in the `n-1`th row.

2. Using this recursive insight:
   - Base case: If `n = 1`, return `0` since the first row is always `0`.
   - Recursive case: Determine the symbol based on the value from the previous row and the position being odd or even.

Here’s a concise implementation:

```python
def kthGrammar(n, k):
    # Base case, first row is always '0'
    if n == 1:
        return 0
    # Recurse to find the symbol in the previous row
    if k % 2 == 1:
        return kthGrammar(n - 1, (k + 1) // 2)
    else:
        return 1 - kthGrammar(n - 1, k // 2)
```

---

**Interviewer**: Excellent, what is the time and space complexity of this optimized approach?

**Interviewee**: 
- **Time Complexity**: Each recursive call reduces the problem size by half, leading to a time complexity of \(O(\log n)\), since the depth of recursion is \(O(\log n)\).
- **Space Complexity**: The space complexity is also \(O(\log n)\), as we need to maintain the stack frames for the recursive calls up to the depth of \(O(\log n)\).

---

**Interviewer**: Great job! This approach is much more efficient. Can you draw a binary tree to help visualize this recursion?

---

**Interviewee**: Sure, let's draw a binary tree to visualize how each row is constructed from the previous one. Each parent node splits into two children where:
- 0 -> 01
- 1 -> 10

Here's a small tree for `n = 3`:
```
    n=1     0
           / \
    n=2   0   1
         /|   |\
    n=3 0 1   1 0
```

From this tree, you can trace any path from the root node down to find the kth symbol in the nth row efficiently using the recursive insight we discussed.

Sure, I'll provide the implementations of the optimized recursive function in each language. The function solves the problem with \(O(\log n)\) time and space complexity. 

### C++
```cpp
class Solution {
public:
    int kthGrammar(int n, int k) {
        if (n == 1) {
            return 0;
        }
        if (k % 2 == 1) {
            return kthGrammar(n - 1, (k + 1) / 2);
        } else {
            return 1 - kthGrammar(n - 1, k / 2);
        }
    }
};
```

### Java
```java
class Solution {
    public int kthGrammar(int n, int k) {
        if (n == 1) {
            return 0;
        }
        if (k % 2 == 1) {
            return kthGrammar(n - 1, (k + 1) / 2);
        } else {
            return 1 - kthGrammar(n - 1, k / 2);
        }
    }
}
```

### Python
```python
class Solution(object):
    def kthGrammar(self, n, k):
        """
        :type n: int
        :type k: int
        :rtype: int
        """
        if n == 1:
            return 0
        if k % 2 == 1:
            return self.kthGrammar(n - 1, (k + 1) // 2)
        else:
            return 1 - self.kthGrammar(n - 1, k // 2)
```

### Python3
```python
class Solution:
    def kthGrammar(self, n: int, k: int) -> int:
        if n == 1:
            return 0
        if k % 2 == 1:
            return self.kthGrammar(n - 1, (k + 1) // 2)
        else:
            return 1 - self.kthGrammar(n - 1, k // 2)
```

### C
```c
int kthGrammar(int n, int k) {
    if (n == 1) {
        return 0;
    }
    if (k % 2 == 1) {
        return kthGrammar(n - 1, (k + 1) / 2);
    } else {
        return 1 - kthGrammar(n - 1, k / 2);
    }
}
```

### C#
```csharp
public class Solution {
    public int KthGrammar(int n, int k) {
        if (n == 1) {
            return 0;
        }
        if (k % 2 == 1) {
            return KthGrammar(n - 1, (k + 1) / 2);
        } else {
            return 1 - KthGrammar(n - 1, k / 2);
        }
    }
}
```

### JavaScript
```javascript
/**
 * @param {number} n
 * @param {number} k
 * @return {number}
 */
var kthGrammar = function(n, k) {
    if (n == 1) {
        return 0;
    }
    if (k % 2 === 1) {
        return kthGrammar(n - 1, Math.ceil(k / 2));
    } else {
        return 1 - kthGrammar(n - 1, Math.ceil(k / 2));
    }
};
```

### TypeScript
```typescript
function kthGrammar(n: number, k: number): number {
    if (n == 1) {
        return 0;
    }
    if (k % 2 === 1) {
        return kthGrammar(n - 1, Math.ceil(k / 2));
    } else {
        return 1 - kthGrammar(n - 1, Math.ceil(k / 2));
    }
}
```

### PHP
```php
class Solution {

    /**
     * @param Integer $n
     * @param Integer $k
     * @return Integer
     */
    function kthGrammar($n, $k) {
        if ($n == 1) {
            return 0;
        }
        if ($k % 2 == 1) {
            return $this->kthGrammar($n - 1, (int)(($k+1) / 2));
        } else {
            return 1 - $this->kthGrammar($n - 1, (int)($k / 2));
        }
    }
}
```

### Swift
```swift
class Solution {
    func kthGrammar(_ n: Int, _ k: Int) -> Int {
        if n == 1 {
            return 0;
        }
        if k % 2 == 1 {
            return kthGrammar(n - 1, (k + 1) / 2);
        } else {
            return 1 - kthGrammar(n - 1, k / 2);
        }
    }
}
```

### Kotlin
```kotlin
class Solution {
    fun kthGrammar(n: Int, k: Int): Int {
        if (n == 1) {
            return 0
        }
        return if (k % 2 == 1) {
            kthGrammar(n - 1, (k + 1) / 2)
        } else {
            1 - kthGrammar(n - 1, k / 2)
        }
    }
}
```

### Dart
```dart
class Solution {
  int kthGrammar(int n, int k) {
    if (n == 1) {
      return 0;
    }
    if (k % 2 == 1) {
      return kthGrammar(n - 1, (k + 1) ~/ 2);
    } else {
      return 1 - kthGrammar(n - 1, k ~/ 2);
    }
  }
}
```

### Go
```go
func kthGrammar(n int, k int) int {
    if n == 1 {
        return 0;
    }
    if k % 2 == 1 {
        return kthGrammar(n - 1, (k + 1) / 2);
    } else {
        return 1 - kthGrammar(n - 1, k / 2);
    }
}
```

### Ruby
```ruby
# @param {Integer} n
# @param {Integer} k
# @return {Integer}
def kth_grammar(n, k)
    if n == 1
        return 0
    end
    if k % 2 == 1
        return kth_grammar(n - 1, (k + 1) / 2)
    else
        return 1 - kth_grammar(n - 1, k / 2)
    end
end
```

### Scala
```scala
object Solution {
    def kthGrammar(n: Int, k: Int): Int = {
        if (n == 1) {
            return 0;
        }
        if (k % 2 == 1) {
            return kthGrammar(n - 1, (k + 1) / 2);
        } else {
            return 1 - kthGrammar(n - 1, k / 2);
        }
    }
}
```

### Rust
```rust
impl Solution {
    pub fn kth_grammar(n: i32, k: i32) -> i32 {
        if n == 1 {
            return 0;
        }
        if k % 2 == 1 {
            return Solution::kth_grammar(n - 1, (k + 1) / 2);
        } else {
            return 1 - Solution::kth_grammar(n - 1, k / 2);
        }
    }
}
```

### Racket
```racket
(define/contract (kth-grammar n k)
  (-> exact-integer? exact-integer? exact-integer?)
  (if (= n 1)
      0
      (if (odd? k)
          (kth-grammar (- n 1) (ceiling (/ (+ k 1) 2)))
          (- 1 (kth-grammar (- n 1) (/ k 2)))))
```

### Erlang
```erlang
-spec kth_grammar(N :: integer(), K :: integer()) -> integer().
kth_grammar(N, K) -> 
    case N of
        1 -> 0;
        _ -> case K rem 2 of
                1 -> kth_grammar(N - 1, (K + 1) div 2);
                0 -> 1 - kth_grammar(N - 1, K div 2)
             end
    end.
```

### Elixir
```elixir
defmodule Solution do
  @spec kth_grammar(n :: integer, k :: integer) :: integer
  def kth_grammar(n, k) do
    if n == 1 do
      0
    else
      if rem(k, 2) == 1 do
        kth_grammar(n - 1, div(k + 1, 2))
      else
        1 - kth_grammar(n - 1, div(k, 2))
      end
    end
  end
end
```


### Closing Statement

**Interviewer**: Great, we've successfully discussed how to solve the problem of finding the `kth` symbol in the `nth` row of a binary grammar sequence generated by specific rules. You correctly described the brute-force approach and its complexities and also arrived at an optimized solution using a recursive approach. This optimization significantly reduces the time and space complexity to \(O(\log n)\), making the solution scalable for larger inputs.

You have implemented the recursive approach in multiple programming languages, demonstrating your ability to adapt the solution across different coding environments. Well done! 

Let’s close this discussion. Do you have any questions about this problem or the approaches we discussed?

**Interviewee**: No, everything is clear. Thank you for the guidance!

**Interviewer**: You're welcome! Great job today, and keep practicing these kinds of problems to sharpen your problem-solving skills.

### Similar Questions

1. **Pascal's Triangle**: Given an integer row index, return the row for Pascal's Triangle.
2. **Gray Code**: Given an integer `n`, generate a sequence of `n`-bit Gray codes.
3. **Recursive Sequence Generation**: Given a rule for generating elements of a sequence, find the `kth` element after `n` generations.
4. **Fibonacci Sequence**: Write an efficient algorithm to determine the `nth` Fibonacci number.
5. **Fractal Pattern Generation**: Generate the `kth` pattern in a fractal sequence based on specific recursive rules.
6. **Nth Tribonacci Number**: Given `n`, find the `nth` number in the tribonacci sequence.
   
Each of these questions enhances your understanding of recursion, sequence generation, and working with patterns, which are essential skills in problem-solving and algorithm design. Keep exploring these problems to deepen your knowledge further.